coq/model/rBPFEncoder.v
@@ -5,63 +5,63 @@ From bpf.model Require Import ebpf rBPFCommType rBPFSyntax.
 
 Import ListNotations.
 
-Definition encode_bpf (v ins: u64) (from size: nat): u64 :=
+Definition encode_bpf (v ins: int64) (from size: nat): int64 :=
   Int64.bitfield_insert (Z.of_nat from) (Z.of_nat size) ins v.
 
-Definition binary_to_u64
-  (opc : u8) (dv : u4) (sv : u4) (off : i16) (imm : i32) : u64 :=
+Definition binary_to_int64
+  (opc : byte) (dv : nat) (sv : nat) (off : word) (imm : int) : int64 :=
   let v1 := encode_bpf (Int64.repr (Byte.unsigned opc)) (Int64.repr 0%Z) 0 8 in
   let v2 := encode_bpf (Int64.repr (Z.of_nat dv)) v1 8 4 in
   let v3 := encode_bpf (Int64.repr (Z.of_nat sv)) v2 12 4 in
   let v4 := encode_bpf (Int64.repr (Word.signed off)) v3 16 16 in
     encode_bpf (Int64.repr (Int.signed imm)) v4 32 32.
 
-Definition rbpf_encoder (ins : bpf_instruction) : list u64 :=
-  let l : list u64 := [] in
+Definition rbpf_encoder (ins : bpf_instruction) : list int64 :=
+  let l : list int64 := [] in
   match ins with
   | BPF_LD_IMM dst imm1 imm2 =>
-      let opc : u8 := Byte.repr 0x18%Z in
-      let dst_i : u4 := bpf_ireg_to_u4 dst in
-      (binary_to_u64 opc dst_i 0 (Word.repr 0%Z) imm1) :: ((binary_to_u64 (Byte.repr 0%Z) 0 0 (Word.repr 0%Z) imm2) :: l)
+      let opc : byte := Byte.repr 0x18%Z in
+      let dst_i : nat := bpf_ireg_to_nat dst in
+      (binary_to_int64 opc dst_i 0 (Word.repr 0%Z) imm1) :: ((binary_to_int64 (Byte.repr 0%Z) 0 0 (Word.repr 0%Z) imm2) :: l)
   | BPF_LDX mc dst src off =>
-      let opc : u8 := Byte.repr (match mc with
+      let opc : byte := Byte.repr (match mc with
                                  | Mint8unsigned => 0x71%Z
                                  | Mint16unsigned => 0x69%Z
                                  | Mint32 => 0x61%Z
                                  | Mint64 => 0x79%Z
                                  | _ => 0x0%Z
                                 end) in
-      let dst_i : u4 := bpf_ireg_to_u4 dst in
-      let src_i : u4 := bpf_ireg_to_u4 src in
-      (binary_to_u64 opc dst_i src_i off (Int.repr 0%Z)) :: (Int64.repr 0%Z) :: l
+      let dst_i : nat := bpf_ireg_to_nat dst in
+      let src_i : nat := bpf_ireg_to_nat src in
+      (binary_to_int64 opc dst_i src_i off (Int.repr 0%Z)) :: (Int64.repr 0%Z) :: l
   | BPF_ST mc dst (SOImm imm) off =>
-      let opc : u8 := Byte.repr (match mc with
+      let opc : byte := Byte.repr (match mc with
                                  | Mint8unsigned => 0x72%Z
                                  | Mint16unsigned => 0x6a%Z
                                  | Mint32 => 0x62%Z
                                  | Mint64 => 0x7a%Z
                                  | _ => 0x0%Z
                                 end) in
-      let dst_i : u4 := bpf_ireg_to_u4 dst in
-      (binary_to_u64 opc dst_i 0 off imm) :: (Int64.repr 0%Z) :: l
+      let dst_i : nat := bpf_ireg_to_nat dst in
+      (binary_to_int64 opc dst_i 0 off imm) :: (Int64.repr 0%Z) :: l
   | BPF_ST mc dst (SOReg src) off =>
-      let opc : u8 := Byte.repr (match mc with
+      let opc : byte := Byte.repr (match mc with
                                  | Mint8unsigned => 0x72%Z
                                  | Mint16unsigned => 0x6a%Z
                                  | Mint32 => 0x62%Z
                                  | Mint64 => 0x7a%Z
                                  | _ => 0x0%Z
                                 end) in
-      let dst_i : u4 := bpf_ireg_to_u4 dst in
-      let src_i : u4 := bpf_ireg_to_u4 src in
-      (binary_to_u64 opc dst_i src_i off (Int.repr 0%Z)) :: (Int64.repr 0%Z) :: l
+      let dst_i : nat := bpf_ireg_to_nat dst in
+      let src_i : nat := bpf_ireg_to_nat src in
+      (binary_to_int64 opc dst_i src_i off (Int.repr 0%Z)) :: (Int64.repr 0%Z) :: l
 
   | BPF_ADD_STK imm => 
-      let opc : u8 := Byte.repr 0x07%Z in
-      (binary_to_u64 opc 11 0 (Word.repr 0%Z) (Int.repr 0%Z)) :: (Int64.repr 0%Z) :: l
+      let opc : byte := Byte.repr 0x07%Z in
+      (binary_to_int64 opc 11 0 (Word.repr 0%Z) (Int.repr 0%Z)) :: (Int64.repr 0%Z) :: l
 
   | BPF_ALU bop dst (SOImm imm) =>
-      let opc : u8 := Byte.repr (match bop with
+      let opc : byte := Byte.repr (match bop with
                                 | BPF_ADD  => 0x04
                                 | BPF_SUB  => 0x14
                                 | BPF_MUL  => 0x24
@@ -75,10 +75,10 @@ Definition rbpf_encoder (ins : bpf_instruction) : list u64 :=
                                 | BPF_MOV  => 0xb4
                                 | BPF_ARSH => 0xc4
                                 end) in
-      let dst_i : u4 := bpf_ireg_to_u4 dst in
-      (binary_to_u64 opc dst_i 0 (Word.repr 0%Z) imm) :: (Int64.repr 0%Z) :: l
+      let dst_i : nat := bpf_ireg_to_nat dst in
+      (binary_to_int64 opc dst_i 0 (Word.repr 0%Z) imm) :: (Int64.repr 0%Z) :: l
   | BPF_ALU bop dst (SOReg src) =>
-      let opc : u8 := Byte.repr (match bop with
+      let opc : byte := Byte.repr (match bop with
                                 | BPF_ADD  => 0x0c
                                 | BPF_SUB  => 0x1c
                                 | BPF_MUL  => 0x2c
@@ -92,26 +92,26 @@ Definition rbpf_encoder (ins : bpf_instruction) : list u64 :=
                                 | BPF_MOV  => 0xbc
                                 | BPF_ARSH => 0xcc
                                 end) in
-      let dst_i : u4 := bpf_ireg_to_u4 dst in
-      let src_i : u4 := bpf_ireg_to_u4 src in
-      (binary_to_u64 opc dst_i src_i (Word.repr 0%Z) (Int.repr 0%Z)) :: (Int64.repr 0%Z) :: l
+      let dst_i : nat := bpf_ireg_to_nat dst in
+      let src_i : nat := bpf_ireg_to_nat src in
+      (binary_to_int64 opc dst_i src_i (Word.repr 0%Z) (Int.repr 0%Z)) :: (Int64.repr 0%Z) :: l
 
   | BPF_NEG32_REG dst =>
-      let opc : u8 := Byte.repr 0x84%Z in
-      let dst_i : u4 := bpf_ireg_to_u4 dst in
-      (binary_to_u64 opc dst_i 0 (Word.repr 0%Z) (Int.repr 0%Z)) :: (Int64.repr 0%Z) :: l
+      let opc : byte := Byte.repr 0x84%Z in
+      let dst_i : nat := bpf_ireg_to_nat dst in
+      (binary_to_int64 opc dst_i 0 (Word.repr 0%Z) (Int.repr 0%Z)) :: (Int64.repr 0%Z) :: l
 
   | BPF_LE dst imm => 
-      let opc : u8 := Byte.repr 0xd4%Z in
-      let dst_i : u4 := bpf_ireg_to_u4 dst in
-      (binary_to_u64 opc dst_i 0 (Word.repr 0%Z) imm) :: (Int64.repr 0%Z) :: l
+      let opc : byte := Byte.repr 0xd4%Z in
+      let dst_i : nat := bpf_ireg_to_nat dst in
+      (binary_to_int64 opc dst_i 0 (Word.repr 0%Z) imm) :: (Int64.repr 0%Z) :: l
   | BPF_BE dst imm => 
-      let opc : u8 := Byte.repr 0xdc%Z in
-      let dst_i : u4 := bpf_ireg_to_u4 dst in
-      (binary_to_u64 opc dst_i 0 (Word.repr 0%Z) imm) :: (Int64.repr 0%Z) :: l
+      let opc : byte := Byte.repr 0xdc%Z in
+      let dst_i : nat := bpf_ireg_to_nat dst in
+      (binary_to_int64 opc dst_i 0 (Word.repr 0%Z) imm) :: (Int64.repr 0%Z) :: l
 
   | BPF_ALU64 bop dst (SOImm imm) =>
-      let opc : u8 := Byte.repr (match bop with
+      let opc : byte := Byte.repr (match bop with
                                 | BPF_ADD  => 0x07
                                 | BPF_SUB  => 0x17
                                 | BPF_MUL  => 0x27
@@ -125,10 +125,10 @@ Definition rbpf_encoder (ins : bpf_instruction) : list u64 :=
                                 | BPF_MOV  => 0xb7
                                 | BPF_ARSH => 0xc7
                                 end) in
-      let dst_i : u4 := bpf_ireg_to_u4 dst in
-      (binary_to_u64 opc dst_i 0 (Word.repr 0%Z) imm) :: (Int64.repr 0%Z) :: l
+      let dst_i : nat := bpf_ireg_to_nat dst in
+      (binary_to_int64 opc dst_i 0 (Word.repr 0%Z) imm) :: (Int64.repr 0%Z) :: l
   | BPF_ALU64 bop dst (SOReg src) =>
-      let opc : u8 := Byte.repr (match bop with
+      let opc : byte := Byte.repr (match bop with
                                 | BPF_ADD  => 0x0f
                                 | BPF_SUB  => 0x1f
                                 | BPF_MUL  => 0x2f
@@ -142,84 +142,84 @@ Definition rbpf_encoder (ins : bpf_instruction) : list u64 :=
                                 | BPF_MOV  => 0xbf
                                 | BPF_ARSH => 0xcf
                                 end) in
-      let dst_i : u4 := bpf_ireg_to_u4 dst in
-      let src_i : u4 := bpf_ireg_to_u4 src in
-      (binary_to_u64 opc dst_i src_i (Word.repr 0%Z) (Int.repr 0%Z)) :: (Int64.repr 0%Z) :: l
+      let dst_i : nat := bpf_ireg_to_nat dst in
+      let src_i : nat := bpf_ireg_to_nat src in
+      (binary_to_int64 opc dst_i src_i (Word.repr 0%Z) (Int.repr 0%Z)) :: (Int64.repr 0%Z) :: l
 
   | BPF_NEG64_REG dst =>
-      let opc : u8 := Byte.repr 0x87%Z in
-      let dst_i : u4 := bpf_ireg_to_u4 dst in
-      (binary_to_u64 opc dst_i 0 (Word.repr 0%Z) (Int.repr 0%Z)) :: (Int64.repr 0%Z) :: l
+      let opc : byte := Byte.repr 0x87%Z in
+      let dst_i : nat := bpf_ireg_to_nat dst in
+      (binary_to_int64 opc dst_i 0 (Word.repr 0%Z) (Int.repr 0%Z)) :: (Int64.repr 0%Z) :: l
 
   | BPF_HOR64_IMM dst imm =>
-      let opc : u8 := Byte.repr 0xf7%Z in
-      let dst_i : u4 := bpf_ireg_to_u4 dst in
-      (binary_to_u64 opc dst_i 0 (Word.repr 0%Z) imm) :: (Int64.repr 0%Z) :: l
+      let opc : byte := Byte.repr 0xf7%Z in
+      let dst_i : nat := bpf_ireg_to_nat dst in
+      (binary_to_int64 opc dst_i 0 (Word.repr 0%Z) imm) :: (Int64.repr 0%Z) :: l
 
   | BPF_PQR pop dst (SOImm imm) =>
-      let opc : u8 := Byte.repr (match pop with
+      let opc : byte := Byte.repr (match pop with
                                 | BPF_LMUL => 0x86
                                 | BPF_UDIV => 0x46
                                 | BPF_UREM => 0x66
                                 | BPF_SDIV => 0xc6
                                 | BPF_SREM => 0xe6
                                 end) in
-      let dst_i : u4 := bpf_ireg_to_u4 dst in
-      (binary_to_u64 opc dst_i 0 (Word.repr 0%Z) imm) :: (Int64.repr 0%Z) :: l
+      let dst_i : nat := bpf_ireg_to_nat dst in
+      (binary_to_int64 opc dst_i 0 (Word.repr 0%Z) imm) :: (Int64.repr 0%Z) :: l
   | BPF_PQR pop dst (SOReg src) =>
-      let opc : u8 := Byte.repr (match pop with
+      let opc : byte := Byte.repr (match pop with
                                 | BPF_LMUL => 0x8e
                                 | BPF_UDIV => 0x4e
                                 | BPF_UREM => 0x6e
                                 | BPF_SDIV => 0xce
                                 | BPF_SREM => 0xee
                                 end) in
-      let dst_i : u4 := bpf_ireg_to_u4 dst in
-      let src_i : u4 := bpf_ireg_to_u4 src in
-      (binary_to_u64 opc dst_i src_i (Word.repr 0%Z) (Int.repr 0%Z)) :: (Int64.repr 0%Z) :: l
+      let dst_i : nat := bpf_ireg_to_nat dst in
+      let src_i : nat := bpf_ireg_to_nat src in
+      (binary_to_int64 opc dst_i src_i (Word.repr 0%Z) (Int.repr 0%Z)) :: (Int64.repr 0%Z) :: l
   | BPF_PQR64 pop dst (SOImm imm) =>
-      let opc : u8 := Byte.repr (match pop with
+      let opc : byte := Byte.repr (match pop with
                                 | BPF_LMUL => 0x96
                                 | BPF_UDIV => 0x56
                                 | BPF_UREM => 0x76
                                 | BPF_SDIV => 0xd6
                                 | BPF_SREM => 0xf6
                                 end) in
-      let dst_i : u4 := bpf_ireg_to_u4 dst in
-      (binary_to_u64 opc dst_i 0 (Word.repr 0%Z) imm) :: (Int64.repr 0%Z) :: l
+      let dst_i : nat := bpf_ireg_to_nat dst in
+      (binary_to_int64 opc dst_i 0 (Word.repr 0%Z) imm) :: (Int64.repr 0%Z) :: l
   | BPF_PQR64 pop dst (SOReg src) =>
-      let opc : u8 := Byte.repr (match pop with
+      let opc : byte := Byte.repr (match pop with
                                 | BPF_LMUL => 0x9e
                                 | BPF_UDIV => 0x5e
                                 | BPF_UREM => 0x7e
                                 | BPF_SDIV => 0xde
                                 | BPF_SREM => 0xfe
                                 end) in
-      let dst_i : u4 := bpf_ireg_to_u4 dst in
-      let src_i : u4 := bpf_ireg_to_u4 src in
-      (binary_to_u64 opc dst_i src_i (Word.repr 0%Z) (Int.repr 0%Z)) :: (Int64.repr 0%Z) :: l
+      let dst_i : nat := bpf_ireg_to_nat dst in
+      let src_i : nat := bpf_ireg_to_nat src in
+      (binary_to_int64 opc dst_i src_i (Word.repr 0%Z) (Int.repr 0%Z)) :: (Int64.repr 0%Z) :: l
   | BPF_PQR2 pop2 dst (SOImm imm) =>
-      let opc : u8 := Byte.repr (match pop2 with
+      let opc : byte := Byte.repr (match pop2 with
                                 | BPF_UHMUL => 0x36
                                 | BPF_SHMUL => 0xb6
                                 end) in
-      let dst_i : u4 := bpf_ireg_to_u4 dst in
-      (binary_to_u64 opc dst_i 0 (Word.repr 0%Z) imm) :: (Int64.repr 0%Z) :: l
+      let dst_i : nat := bpf_ireg_to_nat dst in
+      (binary_to_int64 opc dst_i 0 (Word.repr 0%Z) imm) :: (Int64.repr 0%Z) :: l
   | BPF_PQR2 pop2 dst (SOReg src) =>
-      let opc : u8 := Byte.repr (match pop2 with
+      let opc : byte := Byte.repr (match pop2 with
                                 | BPF_UHMUL => 0x3e
                                 | BPF_SHMUL => 0xbe
                                 end) in
-      let dst_i : u4 := bpf_ireg_to_u4 dst in
-      let src_i : u4 := bpf_ireg_to_u4 src in
-      (binary_to_u64 opc dst_i src_i (Word.repr 0%Z) (Int.repr 0%Z)) :: (Int64.repr 0%Z) :: l
+      let dst_i : nat := bpf_ireg_to_nat dst in
+      let src_i : nat := bpf_ireg_to_nat src in
+      (binary_to_int64 opc dst_i src_i (Word.repr 0%Z) (Int.repr 0%Z)) :: (Int64.repr 0%Z) :: l
 
   | BPF_JA off =>
-      let opc : u8 := Byte.repr 0x05%Z in
-      (binary_to_u64 opc 0 0 off (Int.repr 0%Z)) :: (Int64.repr 0%Z) :: l
+      let opc : byte := Byte.repr 0x05%Z in
+      (binary_to_int64 opc 0 0 off (Int.repr 0%Z)) :: (Int64.repr 0%Z) :: l
 
   | BPF_JUMP cond dst (SOImm imm) off =>
-      let opc : u8 := Byte.repr (match cond with
+      let opc : byte := Byte.repr (match cond with
                                 | Eq  => 0x15
                                 | Gt  => 0x25
                                 | Ge  => 0x35
@@ -232,10 +232,10 @@ Definition rbpf_encoder (ins : bpf_instruction) : list u64 :=
                                 | SLt => 0xc5
                                 | SLe => 0xd5
                                 end) in
-      let dst_i : u4 := bpf_ireg_to_u4 dst in
-      (binary_to_u64 opc dst_i 0 off imm) :: (Int64.repr 0%Z) :: l
+      let dst_i : nat := bpf_ireg_to_nat dst in
+      (binary_to_int64 opc dst_i 0 off imm) :: (Int64.repr 0%Z) :: l
   | BPF_JUMP cond dst (SOReg src) off =>
-      let opc : u8 := Byte.repr (match cond with
+      let opc : byte := Byte.repr (match cond with
                                 | Eq  => 0x1d
                                 | Gt  => 0x2d
                                 | Ge  => 0x3d
@@ -248,22 +248,22 @@ Definition rbpf_encoder (ins : bpf_instruction) : list u64 :=
                                 | SLt => 0xcd
                                 | SLe => 0xdd
                                 end) in
-      let dst_i : u4 := bpf_ireg_to_u4 dst in
-      let src_i : u4 := bpf_ireg_to_u4 src in
-      (binary_to_u64 opc dst_i src_i off (Int.repr 0%Z)) :: (Int64.repr 0%Z) :: l
+      let dst_i : nat := bpf_ireg_to_nat dst in
+      let src_i : nat := bpf_ireg_to_nat src in
+      (binary_to_int64 opc dst_i src_i off (Int.repr 0%Z)) :: (Int64.repr 0%Z) :: l
 
   | BPF_CALL_REG src imm =>
-      let opc : u8 := Byte.repr 0x8d%Z in
-      let src_i : u4 := bpf_ireg_to_u4 src in
-      (binary_to_u64 opc 0 src_i (Word.repr 0%Z) imm) :: (Int64.repr 0%Z) :: l
+      let opc : byte := Byte.repr 0x8d%Z in
+      let src_i : nat := bpf_ireg_to_nat src in
+      (binary_to_int64 opc 0 src_i (Word.repr 0%Z) imm) :: (Int64.repr 0%Z) :: l
   | BPF_CALL_IMM src imm =>
-      let opc : u8 := Byte.repr 0x85%Z in
-      let src_i : u4 := bpf_ireg_to_u4 src in
-      (binary_to_u64 opc 0 src_i (Word.repr 0%Z) imm) :: (Int64.repr 0%Z) :: l
+      let opc : byte := Byte.repr 0x85%Z in
+      let src_i : nat := bpf_ireg_to_nat src in
+      (binary_to_int64 opc 0 src_i (Word.repr 0%Z) imm) :: (Int64.repr 0%Z) :: l
   
   | BPF_EXIT =>
-      let opc : u8 := Byte.repr 0x85%Z in
-      (binary_to_u64 opc 0 0 (Word.repr 0%Z) (Int.repr 0%Z)) :: (Int64.repr 0%Z) :: l
+      let opc : byte := Byte.repr 0x85%Z in
+      (binary_to_int64 opc 0 0 (Word.repr 0%Z) (Int.repr 0%Z)) :: (Int64.repr 0%Z) :: l
   end.
 
 
